{
 "cells": [
  {
   "cell_type": "markdown",
   "id": "95193206",
   "metadata": {},
   "source": [
    "# Task 4\n",
    "\n",
    "### a) \n",
    "\n",
    "Since $B(t)$ is a $C^1$ function we know that it has to be continious and continious differentiable in the interval $t \\in [0, m]$. In other words $B(t)$ has to satisfy the following conditions\n",
    "\n",
    "$$\n",
    "\\begin{cases}\n",
    "p_{3,i} = p_{0,i+1}, & \\forall \\; i = 1, \\ldots, m-1 \\\\\n",
    "p_{3,i} - p_{2,i} = p_{1,i+1} - p_{0,i+1},  & \\forall \\; i = 1, \\ldots, m-1.\n",
    "\\end{cases}\n",
    "$$\n",
    "\n",
    "From the equation above we observe that $p_{2,i}$ can be expressed as\n",
    "\n",
    "$$\n",
    "p_{2,i} = 2p_{0,i+1} - p_{1,i+1}\n",
    "$$\n",
    "\n",
    "We can try and phrase this information using the velocity $v_{i+1}$ at $p_{0,i+1}$. Using the results from $\\textbf{2c)}$ and the equation above we get that\n",
    "\n",
    "$$\n",
    "\\begin{align*}\n",
    "v_{i+1} &= c_{i+1}'(0) \\\\\n",
    "&= 3 (p_{1,i+1}-p_{0,i+1}) \\\\\n",
    "&= 3 \\left(p_{1,i+1} - \\frac{1}{2}(p_{2,i} +  p_{1,i+1})\\right) \\\\\n",
    "&= \\frac{3}{2}\\left(p_{1,i+1} - p_{2,i}\\right)\n",
    "\\end{align*}\n",
    "$$\n",
    "\n",
    "We observe that from this expression we can recover both “neighboring” points $p_{2,i}$ and $p_{1,i+1}$.\n",
    "\n",
    "\n",
    "### b) \n",
    "\n",
    "We want to minimize the (squared) acceleration of the curve\n",
    "\n",
    "$$\n",
    "F(\\mathbf{P}) := \\int_0^m ||\\mathbf{B}''(t)||^2 dt,\n",
    "$$\n",
    "\n",
    "with respect to the remaining control points \n",
    "\n",
    "$$\n",
    "\\mathbf{P} = [p_{0,1},p_{1,1}, p_{0,2}, p_{1,2}, \\ldots , p_{0,m-1}, p_{1,m-1}, p_{0,m}, p_{1,m}, p_{2,m}, p_{3,m}].\n",
    "$$\n",
    "\n",
    "For simplicity we only consider one segment of the composite Bézier curve for the points ($q_0$, $q_1$, $q_2$, $q_3$) $\\in \\mathbb{R}^2$; $b_3(t; q_0, q_1, q_2, q_3)$ and use this to find the gradient of \n",
    "\n",
    "$$\n",
    "\\tilde{F}(q_0,q_1,q_2,q_3) := \\int_0^1 ||b_3''(t;q_0, q_1, q_2, q_3)||_2^2 dt\n",
    "$$\n",
    "\n",
    "with respect to the control points $q_i$, $i = 0, \\ldots, 3$. From task $\\textbf{2c)}$ we recall that\n",
    "\n",
    "$$\n",
    "\\begin{align*}\n",
    "b_3''(t;q_0, q_1, q_2, q_3) &= 3 \\cdot 2 \\left[ \\sum_{i=0}^{3-2} B_{i,3-2}(t)\\left(q_{i+2} - 2q_{i+1} + q_{i}\\right) \\right] \\\\\n",
    "&= 6 \\left[ \\sum_{i=0}^{1} B_{i,1}(t)\\left(q_{i+2} - 2q_{i+1} + q_{i}\\right) \\right] \\\\\n",
    "&= 6 \\left[ B_{0,1}(t)(q_2 -2q_1 + q_0) + B_{1,1}(t)(q_3 -2q_2 + q_1)\\right] \\\\\n",
    "&= 6 \\left[ \\binom{1}{0}t^{0}(1-t)^{1-0}(q_2 -2q_1 + q_0) + \\binom{1}{1}t^{1}(1-t)^{1-1}(q_3 -2q_2 + q_1)\\right] \\\\\n",
    "&= 6 \\left[ (1-t)(q_2 - 2q_1 + q_0) + t(q_3 - 2q_2 + q_1)\\right] \\\\\n",
    "&= 6 \\left[ t(q_3 -3q_2 + 3q_1 - q_0) + q_2 -2q_1 + q_0 \\right] \n",
    "\\end{align*}\n",
    "$$\n",
    "\n",
    "Thus\n",
    "\n",
    "$$\n",
    "\\begin{align*}\n",
    "\\tilde{F}(q_0,q_1,q_2,q_3) &:= \\int_0^1 ||b_3''(t;q_0, q_1, q_2, q_3)||_2^2 dt \\\\\n",
    "&= \\int_0^1 ||6 \\left[ t(q_3 -3q_2 + 3q_1 - q_0) + q_2 -2q_1 + q_0 \\right] ||_2^2 dt \\\\\n",
    "&= 36 \\int_0^1 (q_3 -3q_2 + 3q_1 - q_0)^2 + (q_2 -2q_1 + q_0)^2 dt \\\\\n",
    "&= 36 \\left[ (q_3 -3q_2 + 3q_1 - q_0)^2 + (q_2 -2q_1 + q_0)^2 \\right], \n",
    "\\end{align*}\n",
    "$$\n",
    "\n",
    "and the gradient of $\\tilde{F}(q_0,q_1,q_2,q_3)$ is given by\n",
    "\n",
    "$$\n",
    "\\begin{align*}\n",
    "\\nabla \\tilde{F}(q_0,q_1,q_2,q_3) &= \\left( \\frac{\\partial \\tilde{F}}{\\partial q_0}, \\frac{\\partial \\tilde{F}}{\\partial q_1}, \\frac{\\partial \\tilde{F}}{\\partial q_2}, \\frac{\\partial \\tilde{F}}{\\partial q_3}\\right) \\\\\n",
    "&= 72\\left([2q_0-5q_1+4q_2-q_3], [-5q_0+13q_1-11q_2+3q_3], [4q_0-11q_1+10q_2-3q_3], [-q_0+3q_1-3q_2+q_3]\\right)\n",
    "\\end{align*}\n",
    "$$\n",
    "\n",
    "We can use this result to compute the gradient of $F$. Since $\\mathbf{B}(t)$ is a $C^1$ function we know that it is continous and continiously differentiable. So the missing points $p_{2,i}$ and $p_{3,i}$ using the results from $\\textbf{4a)}$ can be expressed as\n",
    "\n",
    "$$\n",
    "\\begin{cases}\n",
    "p_{2,i} = 2p_{0,i+1} - p_{1,i+1}, && \\forall i = 1, \\ldots, m-1 \\\\\n",
    "p_{3,i} = p_{0,i+1}, && \\forall i = 1, \\ldots, m-1 \n",
    "\\end{cases}\n",
    "$$\n",
    "\n",
    "Then we can express $\\tilde{F}$ for one segment as\n",
    "\n",
    "$$\n",
    "\\begin{align*}\n",
    "\\tilde{F}(p_{0,i}, p_{1,i}, p_{2,i}, p_{3,i}) &:= 36 \\left[ (p_{3,i} -3p_{2,i} + 3p_{1,i} - p_{0,i})^2 + (p_{2,i} -2p_{1,i} + p_{0,i})^2 \\right]\\\\\n",
    "&= 36 \\left[ (p_{0,i+1} -3(2p_{0,i+1} - p_{1,i+1}) + 3p_{1,i} - p_{0,i})^2 + (2p_{0,i+1} - p_{1,i+1} -2p_{1,i} + p_{0,i})^2 \\right] \\\\\n",
    "&= 36 \\left[ (3p_{1,i+1} -5p_{0,i+1} + 3p_{1,i} - p_{0,i})^2 + (2p_{0,i+1} - p_{1,i+1} -2p_{1,i} + p_{0,i})^2 \\right],\n",
    "\\end{align*}\n",
    "$$\n",
    "\n",
    "for all $i = 1, \\ldots, m-1$. Then we can express $F$ as\n",
    "\n",
    "$$\n",
    "\\begin{align*}\n",
    "&F(p_{0,1}, p_{1,1}, \\ldots, p_{3,m}) :=  \\\\\n",
    "&36 \\left[  \\left(\\sum_{i=1}^{m-1}(3p_{1,i+1} -5p_{0,i+1} + 3p_{1,i} - p_{0,i}) + p_{3,m}-3p_{2,m} + 3p_{1,m}-p_{0,m}\\right)^2 + \\left(\\sum_{i=1}^{m-1} (2p_{0,i+1} - p_{1,i+1} -2p_{1,i} + p_{0,i}) +p_{2,m} - 2p_{1,m} + p_{0,m}\\right)^2 \\right].\n",
    "\\end{align*}\n",
    "$$\n",
    "\n",
    "We observe that we can rearrange the sums such that we get a sum only over index $i$:\n",
    "\n",
    "$$\n",
    "\\begin{align*}\n",
    "\\sum_{i=1}^{m-1}(3p_{1,i+1} -5p_{0,i+1} + 3p_{1,i} - p_{0,i}) &= \\sum_{i=1}^{m-1}(3p_{1,i+1} -5p_{0,i+1}) + \\sum_{i=1}^{m-1}(3p_{1,i} - p_{0,i})\\\\\n",
    "&= \\sum_{i=2}^{m-1}(3p_{1,i} -5p_{0,i}) + 3p_{1,m} -5p_{0,m} + 3p_{1,1} - p_{0,1} + \\sum_{i=2}^{m-1}(3p_{1,i} - p_{0,i}) \\\\\n",
    "&= \\sum_{i=2}^{m-1}(3p_{1,i} -5p_{0,i} + 3p_{1,i} - p_{0,i}) + 3p_{1,m} -5p_{0,m} + 3p_{1,1} - p_{0,1} \\\\\n",
    "&= 6 \\sum_{i=2}^{m-1}(p_{1,i} -p_{0,i}) + 3p_{1,m} -5p_{0,m} + 3p_{1,1} - p_{0,1},\n",
    "\\end{align*}\n",
    "$$\n",
    "\n",
    "and \n",
    "\n",
    "$$\n",
    "\\begin{align*}\n",
    "\\sum_{i=1}^{m-1} (2p_{0,i+1} - p_{1,i+1} -2p_{1,i} + p_{0,i}) &= \\sum_{i=1}^{m-1} (2p_{0,i+1} - p_{1,i+1}) + \\sum_{i=1}^{m-1}p_{0,i} -2p_{1,i} \\\\\n",
    "&= \\sum_{i=2}^{m-1} (2p_{0,i} - p_{1,i}) + 2p_{0,m} - p_{1,m} + p_{0,1} -2p_{1,1} + \\sum_{i=2}^{m-1} (p_{0,i} -2p_{1,i}) \\\\\n",
    "&= \\sum_{i=2}^{m-1} (2p_{0,i} - p_{1,i} + p_{0,i} -2p_{1,i}) + 2p_{0,m} - p_{1,m} + p_{0,1} -2p_{1,1} \\\\\n",
    "&= 3 \\sum_{i=2}^{m-1} (p_{0,i} - p_{1,i}) + 2p_{0,m} - p_{1,m} + p_{0,1} -2p_{1,1}\n",
    "\\end{align*}\n",
    "$$\n",
    "\n",
    "Then $F$ simplifies to\n",
    "\n",
    "$$\n",
    "\\begin{align*}\n",
    "F(p_{0,1}, p_{1,1}, \\ldots, p_{3,m}) &:= 36 \\left[ \\left( 6 \\sum_{i=2}^{m-1}(p_{1,i} -p_{0,i}) + 3p_{1,1} - p_{0,1} + 3p_{1,m} -5p_{0,m} + p_{3,m}-3p_{2,m} + 3p_{1,m}-p_{0,m} \\right)^2 \\\\\n",
    "+ \\left(3 \\sum_{i=2}^{m-1} (p_{0,i} - p_{1,i}) + p_{0,1} -2p_{1,1} + 2p_{0,m} - p_{1,m} + p_{2,m} - 2p_{1,m} + p_{0,m}\\right)^2 \\right] \\\\\n",
    "&= 36 \\left[ \\left(- p_{0,1} +  3p_{1,1}  + 6 \\sum_{i=2}^{m}(p_{1,i} -p_{0,i}) -3p_{2,m} + p_{3,m} \\right)^2 + \\left( p_{0,1} -2p_{1,1} + 3 \\sum_{i=2}^{m} (p_{0,i} - p_{1,i}) + p_{2,m}\\right)^2 \\right]\n",
    "\\end{align*}\n",
    "$$\n",
    "\n",
    "Since we know that $\\mathbf{B}(t)$ is continiously differentiable we obtain\n",
    "\n",
    "$$\n",
    "\\begin{align*}\n",
    "\\nabla F(p_{0,1}, p_{1,1}, \\ldots, p_{3,m}) &= \\left( \\frac{\\partial F}{\\partial p_{0,1}}, \\frac{\\partial F}{\\partial p_{1,1}}, \\ldots, \\frac{\\partial F}{\\partial p_{3,m}} \\right) \\\\\n",
    "&= \n",
    "\\end{align*}\n",
    "$$\n",
    "\n",
    "\n",
    "\n",
    "Task: \n",
    "While we do not want to write down the whole gradient of F, sketch how you can\n",
    "use the result of F˜ to compute the gradient of F. Remember that B(t) is continuously\n",
    "differentiable.\n",
    "\n",
    "\n",
    "### c) \n",
    "We try to solve the equation \n",
    "\n",
    "$$\n",
    "\\nabla \\tilde{F}(\\mathbf{q}^*) = 0\n",
    "$$\n",
    "\n",
    "then $\\mathbf{q}^*$ is a possible minimizer for $\\tilde{F}(\\mathbf{q})$. We use our calculated gradient from $\\textbf{4b)}$ and we get that\n",
    "\n",
    "$$\n",
    "\\nabla \\tilde{F}(\\mathbf{q^*}) = 72 \n",
    "\\begin{bmatrix}\n",
    "2 & -5 & 4 & -1\\\\\n",
    "-5 & 13 & -11 & 3 \\\\\n",
    "4 & -11 & 10 & -3 \\\\\n",
    "-1 & 3 & -3 & 1\n",
    "\\end{bmatrix}\n",
    "\\begin{bmatrix}\n",
    "q^*_0 \\\\ q^*_1 \\\\ q^*_2 \\\\ q^*_3\n",
    "\\end{bmatrix}\n",
    "= \\vec{0}\n",
    "$$\n",
    "\n",
    "We reduce the matrix to row echolon form and obtain \n",
    "\n",
    "$$\n",
    "\\begin{bmatrix}\n",
    "1 & 0 & -3 & 2\\\\\n",
    "0 & 1 & -2 & 1 \\\\\n",
    "0 & 0 & 0 & 0 \\\\\n",
    "0 & 0 & 0 & 0\n",
    "\\end{bmatrix}\n",
    "\\begin{bmatrix}\n",
    "q^*_0 \\\\ q^*_1 \\\\ q^*_2 \\\\ q^*_3\n",
    "\\end{bmatrix}\n",
    "= \\vec{0}\n",
    "$$\n",
    "\n",
    "From the row echolon representation above we observe that $q^*_2$ and $q^*_3$ are free variables. Which means that the solution to the equation $\\nabla \\tilde{F}(\\mathbf{q}^*) = 0$ has infinitly many solutions. We let $q^*_2 = r$ and $q^*_3 = s$ for any points $r,s \\in \\mathbb{R}^2$. Then the solution of  $\\tilde{F}(\\mathbf{q}^*) = 0$ is \n",
    "\n",
    "$$\n",
    "\\mathbf{q}^* = \\begin{bmatrix}q^*_0 \\\\ q^*_1 \\\\ q^*_2 \\\\ q^*_3\\end{bmatrix} = \\begin{bmatrix} 3r - 2s \\\\ 2r -s \\\\ r \\\\ s \\end{bmatrix}\n",
    "$$\n",
    "\n",
    "We observe from task $\\textbf{4b)}$ that $\\tilde{F}(\\mathbf{q}) \\geq 0$ for all $\\mathbf{q}$. We want to check if our $\\mathbf{q}^*$ is actually a minimizer for $\\tilde{F}(\\mathbf{q})$ and obtain:\n",
    "\n",
    "$$\n",
    "\\begin{align*}\n",
    "\\tilde{F}(3r-2s,2r-s,r,s) &= 36 \\left[ (s -3r + 3(2r-s) -(3r-2s))^2 + (r -2(2r-s) + (3r-2s))^2 \\right] \\\\\n",
    "&= 36 \\left[ (s -3s + 2s -3r + 6r -3r)^2 + (r -4r+3r +2s -2s)^2 \\right] \\\\\n",
    "&= 36 \\left[ 0 + 0 \\right] \\\\\n",
    "&= 0\n",
    "\\end{align*}\n",
    "$$\n",
    "\n",
    "We observe from the result above that our $\\mathbf{q}^*$ is a global minimizer for the function $\\tilde{F}(q_0,q_1,q_2,q_3)$, since \n",
    "\n",
    "$$\n",
    "\\begin{align*}\n",
    "\\tilde{F}(\\mathbf{q}^*) \\leq \\tilde{F}(\\mathbf{q}), &&\\forall \\mathbf{q}.\n",
    "\\end{align*}\n",
    "$$\n",
    "\n",
    "For the overall problem $F$ we have to take into account the properties of $C^1$ between the segments. For simplicity \n",
    "\n",
    "Task: \n",
    "For the overall problem F we even have to take into account the properties from the C^1\n",
    "property between the segments. What about the solution now? Is it unique? You may\n",
    "argue intuitively here or provide a concrete example of two minimisers for a 2-segment\n",
    "curve, i.e. m = 2.\n",
    "\n",
    "\n",
    "### d)\n",
    "\n",
    "We extend our problem to have some (data) points $\\mathbf{d}_i \\in \\mathbb{R}^2$, $i = 0,\\ldots m$ and we extend the problem to\n",
    "\n",
    "$$\n",
    "G_{\\lambda}(\\mathbf{P}) = \\frac{\\lambda}{2} \\sum_{i=0}^{m} ||\\mathbf{d}_i - \\mathbf{B}(i)||_2^2 + \\int_0^m ||\\mathbf{B}''(t)||_2^2 dt,\n",
    "$$\n",
    "\n",
    "for some $\\lambda > 0$. Again we want to look at the simple case when we only have two points $s,e \\in \\mathbb{R}^2$ and we get that\n",
    "\n",
    "$$\n",
    "\\begin{align*}\n",
    "\\tilde{G}_{\\lambda}(q_0,q_1,q_2,q_3) &= \\frac{\\lambda}{2} \\left(||s - b_3(0;q_0,q_1,q_2,q_3)||_2^2 + ||e - b_3(1;q_0,q_1,q_2,q_3)||_2^2\\right) + \\tilde{F}(q_0,q_1,q_2,q_3) \\\\\n",
    "&= \\frac{\\lambda}{2} \\left(||s - q_0||_2^2 + ||e - q_3||_2^2\\right) + \\tilde{F}(q_0,q_1,q_2,q_3) \n",
    "\\end{align*}\n",
    "$$\n",
    "\n",
    "We recall that $\\tilde{F}(q_0,q_1,q_2,q_3)$ is given by\n",
    "\n",
    "$$\n",
    "\\tilde{F}(q_0,q_1,q_2,q_3) = 36 \\left[ (q_3 -3q_2 + 3q_1 - q_0)^2 + (q_2 -2q_1 + q_0)^2 \\right],\n",
    "$$\n",
    "\n",
    "and that $\\nabla \\tilde{F}(\\mathbf{q}^*) = 0$ had the solution \n",
    "\n",
    "$$\n",
    "\\mathbf{q}_\\tilde{F}^* = \\begin{bmatrix}q^*_0 \\\\ q^*_1 \\\\ q^*_2 \\\\ q^*_3\\end{bmatrix} = \\begin{bmatrix} 3a - 2b \\\\ 2a -b \\\\ a \\\\ b \\end{bmatrix},\n",
    "$$\n",
    "\n",
    "for any points $a,b \\in \\mathbb{R}^2$.\n",
    "Now we will find a minimizer for $\\tilde{G}_{\\lambda}(q_0,q_1,q_2,q_3)$ and determine if this minimizer is unique. We directly see from the equations that $\\tilde{G}_{\\lambda}(q_0,q_1,q_2,q_3)$  has its global minima when $s = q_0$, $e = q_3$ and $\\mathbf{q} = \\mathbf{q}^*_{\\tilde{F}}$. Thus we get that \n",
    "\n",
    "$$\n",
    "\\mathbf{q}^*_{G_{\\lambda}}= \\begin{bmatrix} 3a - 2b \\\\ 2a -b \\\\ a \\\\ b \\end{bmatrix} = \\begin{bmatrix} s \\\\ 2a -b \\\\ a \\\\ e\\end{bmatrix} \n",
    "\\Rightarrow \\begin{cases} q_0 = s = 3a -2b \\\\ q_1 = 2a -b \\\\ q_2 = a \\\\ q_3 = e = b \\end{cases}\n",
    "\\Rightarrow \\begin{cases} a = \\frac{1}{3}(s+ 2e) \\\\ b= e \\end{cases}, \n",
    "$$\n",
    "\n",
    "and we obtain the unique minimizer \n",
    "\n",
    "$$\n",
    "\\mathbf{q}^*_{G_{\\lambda}} = \\begin{bmatrix} s \\\\ \\frac{2}{3}(s + 2e) - e \\\\ \\frac{1}{3}(s+ 2e) \\\\ e \\end{bmatrix} = \n",
    "\\begin{bmatrix} s \\\\ \\frac{1}{3}(2s + e) \\\\ \\frac{1}{3}(s + 2e) \\\\ e \\end{bmatrix} \n",
    "$$\n",
    "\n",
    "If we let $\\lambda$ tend to zero in this model we ignore the first term of the equation and we get \n",
    "\n",
    "$$\n",
    "\\tilde{G}_{\\lambda}(q_0,q_1,q_2,q_3) = \\tilde{F}(q_0,q_1,q_2,q_3), \n",
    "$$\n",
    "\n",
    "and we loose the uniqueness since $\\tilde{F}(q_0,q_1,q_2,q_3)$ has not unique minimizer. When $\\lambda$ tend to $\\infty$ we get \n",
    "\n",
    "$$\n",
    "\\tilde{G}_{\\lambda}(q_0,q_1,q_2,q_3) = \\lim_{\\lambda\\to\\infty} \\frac{\\lambda}{2} \\left(||s - q_0||_2^2 + ||e - q_3||_2^2\\right) + \\tilde{F}(q_0,q_1,q_2,q_3) , \n",
    "$$\n",
    "\n",
    "and we observe that the equation has its global minima when $\\mathbf{q} = \\mathbf{q}^*_{G_{\\lambda}}$. We also observe that if $s \\neq q_0$ or $e \\neq q_3$  $\\tilde{G}_{\\lambda}(q_0,q_1,q_2,q_3)$ also tends to $\\infty$ as $\\lambda \\to \\infty$. \n",
    "\n",
    "For the bigger problem $G_{\\lambda}(\\mathbf{P})$ for $m+1$ (data) points we also have uniqueness. This can be show by induction. \n",
    "\n",
    "$\\textbf{Proof}$: When we have two points we have allready shown that this results in a unique minimizer. For each point $\\mathbf{d}_i$ we add, we get another unique minimizer for the added sequence. Thus for $m+1$ points $\\mathbf{d}_i$ for $i = 0, \\ldots, m$ we have $m$ subsequences $\\tilde{G}_{\\lambda}(q_0,q_1,q_2,q_3)$ from $\\mathbf{d}_i \\to \\mathbf{d}_{i+1}$, $i = 0,\\ldots, m-1$ each with a unique solution. Since $G_{\\lambda}(\\mathbf{P})$ can be written as a linear combination of subsequences $\\tilde{G}_{\\lambda}(q_0,q_1,q_2,q_3)$ with unique minimizers, $G_{\\lambda}(\\mathbf{P})$ also need to have a unique minimizer.\n",
    "\n",
    "If we let $\\lambda \\to 0$ we loose the uniqueness of the minimizer since $G_{0}(\\mathbf{P}) : = F(\\mathbf{P})$ which do not have a unique minimizer. When $\\lambda \\to \\infty$  we still have a unique minimizer for $G_{\\lambda}(\\mathbf{P})$. But if some of the (data) points $\\mathbf{d}_i \\neq p_{0,i+1}$ for $i = 0, \\ldots, m-1$ or $\\mathbf{d}_m \\neq p_{3,m}$, then $G_{\\lambda}(\\mathbf{P})$ also tends to $\\infty$."
   ]
  }
 ],
 "metadata": {
  "kernelspec": {
   "display_name": "Python 3 (ipykernel)",
   "language": "python",
   "name": "python3"
  },
  "language_info": {
   "codemirror_mode": {
    "name": "ipython",
    "version": 3
   },
   "file_extension": ".py",
   "mimetype": "text/x-python",
   "name": "python",
   "nbconvert_exporter": "python",
   "pygments_lexer": "ipython3",
   "version": "3.9.13"
  }
 },
 "nbformat": 4,
 "nbformat_minor": 5
}
