{
 "cells": [
  {
   "cell_type": "code",
   "execution_count": null,
   "id": "2fb2e2fe",
   "metadata": {},
   "outputs": [],
   "source": []
  },
  {
   "cell_type": "markdown",
   "id": "95193206",
   "metadata": {},
   "source": [
    "##### Task 4\n",
    "\n",
    "### a) \n",
    "\n",
    "Since $B(t)$ is a $C^1$ function we know that it has to be continious and continious differentiable in the interval $t \\in [0, m]$. In other words $B(t)$ has to satisfy the following conditions\n",
    "\n",
    "$$\n",
    "\\begin{cases}\n",
    "p_{3,i} = p_{0,i+1}, & \\forall \\; i = 1, \\ldots, m-1 \\\\\n",
    "p_{3,i} - p_{2,i} = p_{1,i+1} - p_{0,i+1},  & \\forall \\; i = 1, \\ldots, m-1.\n",
    "\\end{cases}\n",
    "$$\n",
    "\n",
    "From the equation above we observe that $p_{2,i}$ can be expressed as\n",
    "\n",
    "$$\n",
    "p_{2,i} = 2p_{0,i+1} - p_{1,i+1}\n",
    "$$\n",
    "\n",
    "We can try and phrase this information using the velocity $v_{i+1}$ at $p_{0,i+1}$. Using the results from $\\textbf{2c)}$ and the equation above we get that\n",
    "\n",
    "$$\n",
    "\\begin{align*}\n",
    "v_{i+1} &= c_{i+1}'(0) \\\\\n",
    "&= 3 (p_{1,i+1}-p_{0,i+1}) \\\\\n",
    "&= 3 \\left(p_{1,i+1} - \\frac{1}{2}(p_{2,i} +  p_{1,i+1})\\right) \\\\\n",
    "&= \\frac{3}{2}\\left(p_{1,i+1} - p_{2,i}\\right)\n",
    "\\end{align*}\n",
    "$$\n",
    "\n",
    "We observe that from this expression we can recover both “neighboring” points $p_{2,i}$ and $p_{1,i+1}$.\n",
    "\n",
    "\n",
    "### b) \n",
    "\n",
    "We want to minimize the (squared) acceleration of the curve\n",
    "\n",
    "$$\n",
    "F(\\mathbf{P}) := \\int_0^m ||\\mathbf{B}''(t)||^2 dt,\n",
    "$$\n",
    "\n",
    "with respect to the remaining control points \n",
    "\n",
    "$$\n",
    "\\mathbf{P} = [p_{0,1},p_{1,1}, p_{0,2}, p_{1,2}, \\ldots , p_{0,m-1}, p_{1,m-1}, p_{0,m}, p_{1,m}, p_{2,m}, p_{3,m}].\n",
    "$$\n",
    "\n",
    "For simplicity we only consider one segment of the composite Bézier curve for the points ($q_0$, $q_1$, $q_2$, $q_3$) $\\in \\mathbb{R}^2$; $b_3(t; q_0, q_1, q_2, q_3)$ and use this to find the gradient of \n",
    "\n",
    "$$\n",
    "\\tilde{F}(q_0,q_1,q_2,q_3) := \\int_0^1 ||b_3''(t;q_0, q_1, q_2, q_3)||_2^2 dt\n",
    "$$\n",
    "\n",
    "with respect to the control points $q_i$, $i = 0, \\ldots, 3$. From task $\\textbf{2c)}$ we recall that\n",
    "\n",
    "$$\n",
    "\\begin{align*}\n",
    "b_3''(t;q_0, q_1, q_2, q_3) &= 3 \\cdot 2 \\left[ \\sum_{i=0}^{3-2} B_{i,3-2}(t)\\left(q_{i+2} - 2q_{i+1} + q_{i}\\right) \\right] \\\\\n",
    "&= 6 \\left[ \\sum_{i=0}^{1} B_{i,1}(t)\\left(q_{i+2} - 2q_{i+1} + q_{i}\\right) \\right] \\\\\n",
    "&= 6 \\left[ B_{0,1}(t)(q_2 -2q_1 + q_0) + B_{1,1}(t)(q_3 -2q_2 + q_1)\\right] \\\\\n",
    "&= 6 \\left[ \\binom{1}{0}t^{0}(1-t)^{1-0}(q_2 -2q_1 + q_0) + \\binom{1}{1}t^{1}(1-t)^{1-1}(q_3 -2q_2 + q_1)\\right] \\\\\n",
    "&= 6 \\left[ (1-t)(q_2 - 2q_1 + q_0) + t(q_3 - 2q_2 + q_1)\\right] \\\\\n",
    "&= 6 \\left[ t(q_3 -3q_2 + 3q_1 - q_0) + q_2 -2q_1 + q_0 \\right] \n",
    "\\end{align*}\n",
    "$$\n",
    "\n",
    "Thus\n",
    "\n",
    "$$\n",
    "\\begin{align*}\n",
    "\\tilde{F}(q_0,q_1,q_2,q_3) &:= \\int_0^1 ||b_3''(t;q_0, q_1, q_2, q_3)||_2^2 dt \\\\\n",
    "&= \\int_0^1 ||6 \\left[ t(q_3 -3q_2 + 3q_1 - q_0) + q_2 -2q_1 + q_0 \\right] ||_2^2 dt \\\\\n",
    "&= 36 \\int_0^1 \\left(t(q_3 -3q_2 + 3q_1 - q_0)+q_2 -2q_1 + q_0\\right)^2 dt \\\\,\n",
    "\\end{align*}\n",
    "$$\n",
    "we let $p = (q_3 -3q_2 + 3q_1 - q_0)$ and $r = (q_2 -2q_1 + q_0)$ and we obtain \n",
    "\n",
    "$$\n",
    "\\begin{align*}\n",
    "\\tilde{F}(q_0,q_1,q_2,q_3) &:= 36 \\int_0^1 \\left(tp + r \\right)^2 dt \\\\\n",
    "&= 36 \\int_0^1 t^2 p^2+ 2tpr + r^2 dt \\\\\n",
    "&= 36 \\left[\\frac{1}{3} p^2 t^3 + prt^2  +r^2t\\right]_0^1 \\\\\n",
    "&= 36 \\left(\\frac{1}{3} p^2 + pr  +r^2\\right) \\\\\n",
    "&= 36 \\left(\\frac{1}{3} (q_3 -3q_2 + 3q_1 - q_0)^2 + (q_3 -3q_2 + 3q_1 - q_0)(q_2 -2q_1 + q_0) + (q_2 -2q_1 + q_0)^2 \\right)\\\\\n",
    "&= 12\\left( q_0^2-3q_1q_0 + q_3q_0 + 3q_1^2+3q_2^2+q_3^2-3q_1q_2-3q_2q_3 \\right),\n",
    "\\end{align*}\n",
    "$$\n",
    "\n",
    "and the gradient of $\\tilde{F}(q_0,q_1,q_2,q_3)$ is given by\n",
    "\n",
    "$$\n",
    "\\begin{align*}\n",
    "\\nabla \\tilde{F}(q_0,q_1,q_2,q_3) &= \\left( \\frac{\\partial \\tilde{F}}{\\partial q_0}, \\frac{\\partial \\tilde{F}}{\\partial q_1}, \\frac{\\partial \\tilde{F}}{\\partial q_2}, \\frac{\\partial \\tilde{F}}{\\partial q_3}\\right) \\\\\n",
    "&= 12\\left([2q_0-3q_1+q_3], [-3q_0+6q_1-3q_2], [-3q_1+6q_2-3q_3], [q_0 -3q_2+2q_3]\\right) \\\\\n",
    "&= 12\\begin{bmatrix} \n",
    "2 & -3 & 0 & 1 \\\\\n",
    "-3 & 6 & -3 & 0 \\\\\n",
    "0 & -3 & 6 & -3 \\\\\n",
    "1 & 0 & -3 & 2\n",
    "\\end{bmatrix}\n",
    "\\begin{bmatrix} q_0 \\\\ q_1 \\\\ q_2 \\\\ q3 \\end{bmatrix}\n",
    "\\end{align*}\n",
    "$$\n",
    "\n",
    "We can use this result to compute the whole gradient of $F$ based on the compressed $\\mathbf{P} = [p_{0,1},p_{1,1},p_{0,2}, p_{1,2}, \\ldots , p_{0,m-1}, p_{1,m-1}, p_{0,m}, p_{1,m},p_{2,m}, p_{3,m}]$. From task $\\textbf{4a)}$ we know that the missing points in sequence $c_i$ for $i= 1,\\ldots, m-1$ can be expressed using the first two points in the next sequence. We obtain that $\\tilde{F}_i(p_{0,i}, p_{1,i},p_{2,i}, p_{3,i}) = \\tilde{F}_i(p_{0,i}, p_{1,i},2p_{0,i+1}-p_{1,i+1}, p_{0,i+1})$. Using this and the linearity of the $\\nabla$ operator we get that\n",
    "\n",
    "\n",
    "\n",
    "$$\n",
    "\\begin{align*}\n",
    "\\nabla F(p_{0,1}, p_{1,1}, \\ldots, p_{3,m}) &= \\left( \\frac{\\partial F}{\\partial p_{0,1}}, \\frac{\\partial F}{\\partial p_{1,1}}, \\ldots, \\frac{\\partial F}{\\partial p_{3,m}} \\right) \\\\\n",
    "&= \\left( \\frac{\\partial \\tilde{F_1}}{\\partial p_{0,1}}, \\frac{\\partial \\tilde{F_1}}{\\partial p_{1,1}}, \\ldots, \\frac{\\partial \\tilde{F_m}}{\\partial p_{3,m}} \\right)\n",
    "\\end{align*}\n",
    "$$\n",
    "\n",
    "\n",
    "\n",
    "Task: \n",
    "While we do not want to write down the whole gradient of F, sketch how you can\n",
    "use the result of F˜ to compute the gradient of F. Remember that B(t) is continuously\n",
    "differentiable.\n",
    "\n",
    "\n",
    "### c) \n",
    "We try to solve the equation \n",
    "\n",
    "$$\n",
    "\\nabla \\tilde{F}(\\mathbf{q}^*) = 0\n",
    "$$\n",
    "\n",
    "then $\\mathbf{q}^*$ is a possible minimizer for $\\tilde{F}(\\mathbf{q})$. We use our calculated gradient from $\\textbf{4b)}$ and we get that\n",
    "\n",
    "$$\n",
    "\\nabla \\tilde{F}(\\mathbf{q^*}) = 12\\begin{bmatrix} \n",
    "2 & -3 & 0 & 1 \\\\\n",
    "-3 & 6 & -3 & 0 \\\\\n",
    "0 & -3 & 6 & -3 \\\\\n",
    "1 & 0 & -3 & 2\n",
    "\\end{bmatrix}\n",
    "\\begin{bmatrix}\n",
    "q^*_0 \\\\ q^*_1 \\\\ q^*_2 \\\\ q^*_3\n",
    "\\end{bmatrix}\n",
    "= \\vec{0}\n",
    "$$\n",
    "\n",
    "We reduce the matrix to row echolon form and obtain \n",
    "\n",
    "$$\n",
    "\\begin{bmatrix}\n",
    "1 & 0 & -3 & 2\\\\\n",
    "0 & 1 & -2 & 1 \\\\\n",
    "0 & 0 & 0 & 0 \\\\\n",
    "0 & 0 & 0 & 0\n",
    "\\end{bmatrix}\n",
    "\\begin{bmatrix}\n",
    "q^*_0 \\\\ q^*_1 \\\\ q^*_2 \\\\ q^*_3\n",
    "\\end{bmatrix}\n",
    "= \\vec{0}\n",
    "$$\n",
    "\n",
    "From the row echolon representation above we observe that $q^*_2$ and $q^*_3$ are free variables. Which means that the solution to the equation $\\nabla \\tilde{F}(\\mathbf{q}^*) = 0$ has infinitly many solutions. We let $q^*_2 = r$ and $q^*_3 = s$ for any points $r,s \\in \\mathbb{R}^2$. Then the solution of  $\\tilde{F}(\\mathbf{q}^*) = 0$ is \n",
    "\n",
    "$$\n",
    "\\mathbf{q}^* = \\begin{bmatrix}q^*_0 \\\\ q^*_1 \\\\ q^*_2 \\\\ q^*_3\\end{bmatrix} = \\begin{bmatrix} 3r - 2s \\\\ 2r -s \\\\ r \\\\ s \\end{bmatrix}\n",
    "$$\n",
    "\n",
    "We observe from task $\\textbf{4b)}$ that $\\tilde{F}(\\mathbf{q}) \\geq 0$ for all $\\mathbf{q}$. We want to check if our $\\mathbf{q}^*$ is actually a minimizer for $\\tilde{F}(\\mathbf{q})$ and obtain:\n",
    "\n",
    "$$\n",
    "\\begin{align*}\n",
    "&\\tilde{F}(3r-2s,2r-s,r,s) \\\\\n",
    "&= 36 \\left(\\frac{1}{3} (s -3r + 3(2r-s) - (3r-2s))^2 + (s -3r + 3(2r-s)- (3r-2s))(r -2(2r-s) + (3r-2s)) + (r -2(2r-s) + (3r-2s))^2 \\right)\\\\\n",
    "&= 36 \\left(\\frac{1}{3} (s-3s+2s -3r+6r-3r)^2 + (s-3s+2s -3r+6r-3r)(2s-2s + r-4r+3r) + (2s-2s +r-4r+3r)^2 \\right)\\\\\n",
    "&= 36 \\left( 0 + 0\\cdot 0 + 0 \\right) \\\\\n",
    "&= 0\n",
    "\\end{align*}\n",
    "$$\n",
    "\n",
    "We observe from the result above that our $\\mathbf{q}^*$ is a global minimizer for the function $\\tilde{F}(q_0,q_1,q_2,q_3)$, since \n",
    "\n",
    "$$\n",
    "\\begin{align*}\n",
    "\\tilde{F}(\\mathbf{q}^*) \\leq \\tilde{F}(\\mathbf{q}), &&\\forall \\mathbf{q}.\n",
    "\\end{align*}\n",
    "$$\n",
    "\n",
    "For the overall problem $F$ we have to take into account the properties of $C^1$ between the segments. For simplicity \n",
    "\n",
    "Task: \n",
    "For the overall problem F we even have to take into account the properties from the C^1\n",
    "property between the segments. What about the solution now? Is it unique? You may\n",
    "argue intuitively here or provide a concrete example of two minimisers for a 2-segment\n",
    "curve, i.e. m = 2.\n",
    "\n",
    "\n",
    "### d)\n",
    "\n",
    "We extend our problem to have some (data) points $\\mathbf{d}_i \\in \\mathbb{R}^2$, $i = 0,\\ldots m$ and we extend the problem to\n",
    "\n",
    "$$\n",
    "G_{\\lambda}(\\mathbf{P}) = \\frac{\\lambda}{2} \\sum_{i=0}^{m} ||\\mathbf{d}_i - \\mathbf{B}(i)||_2^2 + \\int_0^m ||\\mathbf{B}''(t)||_2^2 dt,\n",
    "$$\n",
    "\n",
    "for some $\\lambda > 0$. Again we want to look at the simple case when we only have two points $s,e \\in \\mathbb{R}^2$ and we get that\n",
    "\n",
    "$$\n",
    "\\begin{align*}\n",
    "\\tilde{G}_{\\lambda}(q_0,q_1,q_2,q_3) &= \\frac{\\lambda}{2} \\left(||s - b_3(0;q_0,q_1,q_2,q_3)||_2^2 + ||e - b_3(1;q_0,q_1,q_2,q_3)||_2^2\\right) + \\tilde{F}(q_0,q_1,q_2,q_3) \\\\\n",
    "&= \\frac{\\lambda}{2} \\left(||s - q_0||_2^2 + ||e - q_3||_2^2\\right) + \\tilde{F}(q_0,q_1,q_2,q_3) \n",
    "\\end{align*}\n",
    "$$\n",
    "\n",
    "We recall that $\\tilde{F}(q_0,q_1,q_2,q_3)$ is given by\n",
    "\n",
    "$$\n",
    "\\tilde{F}(q_0,q_1,q_2,q_3) = 36 \\left[ |q_3 -3q_2 + 3q_1 - q_0|^2 + |q_2 -2q_1 + q_0|^2 \\right],\n",
    "$$\n",
    "\n",
    "and that $\\nabla \\tilde{F}(\\mathbf{q}^*) = 0$ had the solution \n",
    "\n",
    "$$\n",
    "\\mathbf{q}_\\tilde{F}^* = \\begin{bmatrix}q^*_0 \\\\ q^*_1 \\\\ q^*_2 \\\\ q^*_3\\end{bmatrix} = \\begin{bmatrix} 3a - 2b \\\\ 2a -b \\\\ a \\\\ b \\end{bmatrix},\n",
    "$$\n",
    "\n",
    "for any points $a,b \\in \\mathbb{R}^2$.\n",
    "Now we will find a minimizer for $\\tilde{G}_{\\lambda}(q_0,q_1,q_2,q_3)$ and determine if this minimizer is unique. We directly see from the equations that $\\tilde{G}_{\\lambda}(q_0,q_1,q_2,q_3)$  has its global minima when $s = q_0$, $e = q_3$ and $\\mathbf{q} = \\mathbf{q}^*_{\\tilde{F}}$. Thus we get that \n",
    "\n",
    "$$\n",
    "\\mathbf{q}^*_{G_{\\lambda}}= \\begin{bmatrix} 3a - 2b \\\\ 2a -b \\\\ a \\\\ b \\end{bmatrix} = \\begin{bmatrix} s \\\\ 2a -b \\\\ a \\\\ e\\end{bmatrix} \n",
    "\\Rightarrow \\begin{cases} q_0 = s = 3a -2b \\\\ q_1 = 2a -b \\\\ q_2 = a \\\\ q_3 = e = b \\end{cases}\n",
    "\\Rightarrow \\begin{cases} a = \\frac{1}{3}(s+ 2e) \\\\ b= e \\end{cases}, \n",
    "$$\n",
    "\n",
    "and we obtain the unique minimizer \n",
    "\n",
    "$$\n",
    "\\mathbf{q}^*_{G_{\\lambda}} = \\begin{bmatrix} s \\\\ \\frac{2}{3}(s + 2e) - e \\\\ \\frac{1}{3}(s+ 2e) \\\\ e \\end{bmatrix} = \n",
    "\\begin{bmatrix} s \\\\ \\frac{1}{3}(2s + e) \\\\ \\frac{1}{3}(s + 2e) \\\\ e \\end{bmatrix} \n",
    "$$\n",
    "\n",
    "If we let $\\lambda$ tend to zero in this model we ignore the first term of the equation and we get \n",
    "\n",
    "$$\n",
    "\\tilde{G}_{\\lambda}(q_0,q_1,q_2,q_3) = \\tilde{F}(q_0,q_1,q_2,q_3), \n",
    "$$\n",
    "\n",
    "and we loose the uniqueness since $\\tilde{F}(q_0,q_1,q_2,q_3)$ has not unique minimizer. When $\\lambda$ tend to $\\infty$ we get \n",
    "\n",
    "$$\n",
    "\\tilde{G}_{\\lambda}(q_0,q_1,q_2,q_3) = \\lim_{\\lambda\\to\\infty} \\frac{\\lambda}{2} \\left(||s - q_0||_2^2 + ||e - q_3||_2^2\\right) + \\tilde{F}(q_0,q_1,q_2,q_3) , \n",
    "$$\n",
    "\n",
    "and we observe that the equation has its global minima when $\\mathbf{q} = \\mathbf{q}^*_{G_{\\lambda}}$. We also observe that if $s \\neq q_0$ or $e \\neq q_3$  $\\tilde{G}_{\\lambda}(q_0,q_1,q_2,q_3)$ also tends to $\\infty$ as $\\lambda \\to \\infty$. \n",
    "\n",
    "For the bigger problem $G_{\\lambda}(\\mathbf{P})$ for $m+1$ (data) points we also have uniqueness. This can be shown by induction. \n",
    "\n",
    "$\\textbf{Proof}$: When we have two points we have allready shown that this results in a unique minimizer. For each point $\\mathbf{d}_i$ we add, we get another unique minimizer for the added sequence. Thus for $m+1$ points $\\mathbf{d}_i$ for $i = 0, \\ldots, m$ we have $m$ subsequences $\\tilde{G}_{\\lambda}(q_0,q_1,q_2,q_3)$ from $\\mathbf{d}_i \\to \\mathbf{d}_{i+1}$, $i = 0,\\ldots, m-1$ each with a unique solution. Since $G_{\\lambda}(\\mathbf{P})$ can be written as a linear combination of subsequences $\\tilde{G}_{\\lambda}(q_0,q_1,q_2,q_3)$ with unique minimizers, $G_{\\lambda}(\\mathbf{P})$ also need to have a unique minimizer.\n",
    "\n",
    "If we let $\\lambda \\to 0$ we loose the uniqueness of the minimizer since $G_{0}(\\mathbf{P}) : = F(\\mathbf{P})$ which do not have a unique minimizer. When $\\lambda \\to \\infty$  we still have a unique minimizer for $G_{\\lambda}(\\mathbf{P})$. But if some of the (data) points $\\mathbf{d}_i \\neq p_{0,i+1}$ for $i = 0, \\ldots, m-1$ or $\\mathbf{d}_m \\neq p_{3,m}$, then $G_{\\lambda}(\\mathbf{P})$ also tends to $\\infty$."
   ]
  },
  {
   "cell_type": "markdown",
   "id": "6a7c15e5",
   "metadata": {},
   "source": [
    "### e) \n",
    "\n",
    "Now we want to find a gradient descent method to minimize our function $G_{\\lambda}(\\mathbf{P})$ where we use the $\\mathbf{P}$ from task $\\textbf{3)}$.\n"
   ]
  },
  {
   "cell_type": "code",
   "execution_count": 56,
   "id": "51ba0bf8",
   "metadata": {},
   "outputs": [
    {
     "name": "stdout",
     "output_type": "stream",
     "text": [
      "[[-1.          0.        ]\n",
      " [-1.          0.33333333]\n",
      " [ 1.          0.        ]\n",
      " [ 1.         -0.33333333]\n",
      " [ 0.33333333 -1.        ]\n",
      " [ 0.         -1.        ]]\n",
      "[[ 12.   0.]\n",
      " [-24. -12.]\n",
      " [  0. -12.]\n",
      " [-12.  24.]\n",
      " [-12.   0.]\n",
      " [ 24.  12.]\n",
      " [-12. -24.]\n",
      " [  0.  12.]]\n",
      "[[ 12.   0.]\n",
      " [-24. -12.]\n",
      " [  0. -12.]\n",
      " [-12.  24.]\n",
      " [-12.   0.]\n",
      " [ 24.  12.]\n",
      " [-12. -24.]\n",
      " [  0.  12.]]\n",
      "(array([[ 0.58065569,  1.52921016],\n",
      "       [ 1.06022342,  1.45372845],\n",
      "       [ 1.53018607,  1.02683002],\n",
      "       [ 1.47205427,  0.67326451],\n",
      "       [ 1.07208621, -0.03041954],\n",
      "       [ 0.72642495, -0.37896773],\n",
      "       [ 0.37896773, -0.72642495],\n",
      "       [ 0.03041954, -1.07208621]]), 50)\n",
      "(array([[ 1.06250000e+00,  1.50000000e+00],\n",
      "       [ 1.32291667e+00,  1.41666667e+00],\n",
      "       [ 1.50000000e+00,  1.00000000e+00],\n",
      "       [ 1.41666667e+00,  6.66666667e-01],\n",
      "       [ 1.00000000e+00, -1.15729754e-15],\n",
      "       [ 6.66666667e-01, -3.33333333e-01],\n",
      "       [ 3.33333333e-01, -6.66666667e-01],\n",
      "       [ 2.15212463e-15, -1.00000000e+00]]), 100000)\n"
     ]
    }
   ],
   "source": [
    "import numpy as np\n",
    "\n",
    "# Takes parameters:\n",
    "# 𝜆: parameter for G\n",
    "# P: remaining data points\n",
    "P = np.array([[-1, 0], [-1, 1 / 3], [0, 1], [1 / 3, 1], [1, 0], [1, -1 / 3], [1 / 3, -1], [0, -1]])  \n",
    "\n",
    "def gradient_F_tilde(q):\n",
    "    return 12*np.array([2*q[0]-3*q[1]+q[3], -3*q[0]+6*q[1]-3*q[2], -3*q[1]+6*q[2]-3*q[3], q[0] -3*q[2]+2*q[3]])\n",
    "\n",
    "def compress_P(P_full):\n",
    "    c_P = []\n",
    "    for i in range(0, len(P_full)-4, 4):\n",
    "        c_P.append(P_full[i])\n",
    "        c_P.append(P_full[i+1])\n",
    "    c_P.append(P_full[-4])\n",
    "    c_P.append(P_full[-3])\n",
    "    c_P.append(P_full[-2])\n",
    "    c_P.append(P_full[-1])\n",
    "    return np.array(c_P)\n",
    "\n",
    "\n",
    "def gradient_F(P):\n",
    "    gradient = np.zeros_like(P)\n",
    "    for i in range(0, len(P)-4,2):\n",
    "        g_F_tilde = gradient_F_tilde(np.array([P[i],P[i+1],2*P[i+2]-P[i+3], P[i+2]]))\n",
    "        gradient[i] = g_F_tilde[0]\n",
    "        gradient[i+1] = g_F_tilde[1]\n",
    "    g_F_tilde = gradient_F_tilde(np.array([P[-4],P[-3],P[-2], P[-1]]))\n",
    "    gradient[-4],gradient[-3], gradient[-2], gradient[-1]  = g_F_tilde[0], g_F_tilde[1], g_F_tilde[2], g_F_tilde[3]\n",
    "    return gradient\n",
    "\n",
    "\n",
    "def gradient_G(D,P,𝜆): \n",
    "    gradient_G_F = gradient_F(P)\n",
    "    gradient_norm = np.zeros_like(P)\n",
    "    for i in range(0, len(P)-2,2):\n",
    "        gradient_norm[i] = 𝜆*(P[i]-D[i])\n",
    "    gradient_norm[-1] = 𝜆*(P[-1]-D[-1])\n",
    "    return gradient_norm + gradient_G_F\n",
    "\n",
    "def GD(P, 𝜆, tol, maxiter):\n",
    "    D = P\n",
    "    𝛼 = 0.01  # Step size\n",
    "    d = gradient_G(D,P,𝜆)\n",
    "    norm = np.linalg.norm(-d)\n",
    "    P_new = P + 𝛼*d\n",
    "    it = 0\n",
    "    while it < maxiter:\n",
    "        d_new = -gradient_G(D, P_new,𝜆)\n",
    "        P_new += 𝛼 * d_new\n",
    "        norm = np.linalg.norm(-d_new)\n",
    "        it += 1\n",
    "    return P_new, it\n",
    "      \n",
    "print(compress_P(P))\n",
    "print(gradient_F(P))\n",
    "print(gradient_G(np.copy(P),P,2))\n",
    "\n",
    "print(GD(P, 2, 3, 50))\n",
    "print(GD(P, 2, 3, 100000))\n",
    "\n"
   ]
  },
  {
   "cell_type": "code",
   "execution_count": 2,
   "id": "eceb9bb1",
   "metadata": {},
   "outputs": [],
   "source": [
    "\n",
    "# # Returns value of second term\n",
    "# def F(P):\n",
    "#     n = len(P)\n",
    "#     sum_1 = 0\n",
    "#     sum_2 = 0\n",
    "#     for i in range(2, n - 2, 2):\n",
    "#         sum_1 += 6 * (P[i + 1] - P[i])\n",
    "#         sum_2 += 3 * (P[i] - P[i + 1])\n",
    "#     return 36 * (norm(-P[0] + 3 * P[1] + sum_1 - 3 * P[-2] + P[-1]) ** 2 + norm(P[0] - 2 * P[1] + sum_2 + P[-2]) ** 2)\n",
    "\n",
    "# #Returns value of G\n",
    "# def G(P, 𝜆):\n",
    "#     #Norm of all the elements to p_{1,m-1}\n",
    "#     sum_norm = 0\n",
    "#     for i in range(0, int(len(P) // 2 - 1)):\n",
    "#         for j in range(len(P)):\n",
    "#             if i <= j < 2 * i:\n",
    "#                 sum_norm += norm(P[j] - P[i*2]) ** 2\n",
    "                \n",
    "#     #Adding the norm of the last elements\n",
    "#     sum_norm += norm(P[-4] - P[-1])**2 + norm(P[-3] - P[-1])**2 + norm(P[-2] - P[-1])**2\n",
    "#     return (𝜆 / 2) * sum_norm + F(P)\n",
    "\n",
    "# def gradient_G(P,𝜆): \n",
    "#     d = np.zeros_like(P)\n",
    "#     P_plus_h = P.copy()\n",
    "#     h = 0.1\n",
    "#     for i in range(len(P)):\n",
    "#         for j in range(len(P[i])):\n",
    "#             P_plus_h[i][j] += h\n",
    "#             d[i][j] = (G(P_plus_h, 𝜆) - G(P, 𝜆))/ h  #Calculate appriximate gradient\n",
    "#     return d\n",
    "\n",
    "# #  Calculates the gradient descent for our points P\n",
    "# \n",
    "\n",
    "\n",
    "\n",
    "\n",
    "# result, iterations = GD(P, 𝜆=2, tol=1, maxiter = 6)\n",
    "# print(\"Result:\", result)\n",
    "# print(\"Iterations:\", iterations)\n",
    "        "
   ]
  },
  {
   "cell_type": "code",
   "execution_count": null,
   "id": "6d0a9a20",
   "metadata": {},
   "outputs": [],
   "source": []
  }
 ],
 "metadata": {
  "kernelspec": {
   "display_name": "Python 3 (ipykernel)",
   "language": "python",
   "name": "python3"
  },
  "language_info": {
   "codemirror_mode": {
    "name": "ipython",
    "version": 3
   },
   "file_extension": ".py",
   "mimetype": "text/x-python",
   "name": "python",
   "nbconvert_exporter": "python",
   "pygments_lexer": "ipython3",
   "version": "3.9.13"
  }
 },
 "nbformat": 4,
 "nbformat_minor": 5
}
